Lean4Lean/Instantiate.lean
@@ -1,8 +1,9 @@
 import Lean.Expr
 
 namespace Lean
+namespace Expr
 
-def Expr.cheapBetaReduce (e : Expr) : Expr := Id.run do
+def cheapBetaReduce (e : Expr) : Expr := Id.run do
   if !e.isApp then return e
   let fn := e.getAppFn
   if !fn.isLambda then return e
@@ -18,7 +19,59 @@ def Expr.cheapBetaReduce (e : Expr) : Expr := Id.run do
   let rec loop i fn : Id Expr :=
     if i < args.size then
       match fn with
-      | .lam _ _ dom .. => loop (i + 1) dom
+      | .lam _ _ body .. => loop (i + 1) body
       | _ => cont i fn
     else cont i fn
   loop 0 fn
+
+/--
+Instantiates loose bound variable `0` in `e` using the expression `subst`,
+where in particular a loose `Expr.bvar i` at binding depth `d` is instantiated with `subst` if `i = d`,
+and otherwise it is replaced with `Expr.bvar (i - 1)`; non-loose bound variables are not touched.
+-/
+@[implemented_by instantiate1]
+def instantiate1' (e : @& Expr) (subst : @& Expr) : Expr :=
+  go e 0
+where
+  go : Expr → Nat → Expr
+  | e@(.bvar i), d => if i < d then e else if i = d then subst.liftLooseBVars 0 d else .bvar (i - 1)
+  | .mdata m e, d => .mdata m (go e d)
+  | .proj s i e, d => .proj s i (go e d)
+  | .app f a, d => .app (go f d) (go a d)
+  | .lam n t b bi, d => .lam n (go t d) (go b (d+1)) bi
+  | .forallE n t b bi, d => .forallE n (go t d) (go b (d+1)) bi
+  | .letE n t v b bi, d => .letE n (go t d) (go v d) (go b (d+1)) bi
+  | e@(.const ..), _
+  | e@(.sort _), _
+  | e@(.fvar _), _
+  | e@(.mvar _), _
+  | e@(.lit _), _ => e
+
+/--
+Instantiates the loose bound variables in `e` using the `subst` array,
+where a loose `Expr.bvar i` at "binding depth" `d` is instantiated with `subst[i - d]` if `0 <= i - d < subst.size`,
+and otherwise it is replaced with `Expr.bvar (i - subst.size)`; non-loose bound variables are not touched.
+-/
+@[implemented_by instantiate]
+def instantiate' (e : @& Expr) (subst : @& Array Expr) : Expr :=
+  go e subst.toList
+where
+  go : Expr → List Expr → Expr
+  | e, [] => e
+  | e, a :: as => go (e.instantiate1' a) as
+
+@[implemented_by instantiateRev]
+def instantiateRev' (e : @& Expr) (subst : @& Array Expr) : Expr :=
+  e.instantiate' subst.reverse
+
+@[implemented_by instantiateRange]
+def instantiateRange' (e : @& Expr) (beginIdx endIdx : @& Nat) (subst : @& Array Expr) : Expr :=
+  e.instantiate' (subst.extract beginIdx endIdx)
+
+@[implemented_by instantiateRevRange]
+def instantiateRevRange' (e : @& Expr) (beginIdx endIdx : @& Nat) (subst : @& Array Expr) : Expr :=
+  e.instantiateRev' (subst.extract beginIdx endIdx)
+
+theorem instantiateRev_push {e : Expr} {subst a} :
+    instantiateRev' e (subst.push a) = instantiateRev' (e.instantiate1' a) subst := by
+  let ⟨subst⟩ := subst; simp [instantiateRev', instantiate', instantiate'.go]
