Lean4Lean/TypeChecker.lean
@@ -113,22 +113,22 @@ def inferType (e : Expr) (inferOnly := true) : RecM Expr := fun m => m.inferType
 def inferLambda (e : Expr) (inferOnly : Bool) : RecM Expr := loop #[] e where
   loop fvars : Expr → RecM Expr
   | .lam name dom body bi => do
-    let d := dom.instantiateRev fvars
+    let d := dom.instantiateRev' fvars
+    if !inferOnly then
+      _ ← ensureSortCore (← inferType d inferOnly) d
     let id := ⟨← mkFreshId⟩
     withLCtx ((← getLCtx).mkLocalDecl id name d bi) do
       let fvars := fvars.push (.fvar id)
-      if !inferOnly then
-        _ ← ensureSortCore (← inferType d inferOnly) d
       loop fvars body
   | e => do
-    let r ← inferType (e.instantiateRev fvars) inferOnly
+    let r ← inferType (e.instantiateRev' fvars) inferOnly
     let r := r.cheapBetaReduce
     return (← getLCtx).mkForall fvars r
 
 def inferForall (e : Expr) (inferOnly : Bool) : RecM Expr := loop #[] #[] e where
   loop fvars us : Expr → RecM Expr
   | .forallE name dom body bi => do
-    let d := dom.instantiateRev fvars
+    let d := dom.instantiateRev' fvars
     let t1 ← ensureSortCore (← inferType d inferOnly) d
     let us := us.push t1.sortLevel!
     let id := ⟨← mkFreshId⟩
@@ -136,7 +136,7 @@ def inferForall (e : Expr) (inferOnly : Bool) : RecM Expr := loop #[] #[] e wher
       let fvars := fvars.push (.fvar id)
       loop fvars us body
   | e => do
-    let r ← inferType (e.instantiateRev fvars) inferOnly
+    let r ← inferType (e.instantiateRev' fvars) inferOnly
     let s ← ensureSortCore r e
     return .sort <| us.foldr mkLevelIMax' s.sortLevel!
 
@@ -157,10 +157,10 @@ def inferApp (e : Expr) : RecM Expr := do
     | .forallE _ _ body _ =>
       fType := body
     | _ =>
-      fType := fType.instantiateRevRange j i args
+      fType := fType.instantiateRevRange' j i args
       fType := (← ensureForallCore fType e).bindingBody!
       j := i
-  return fType.instantiateRevRange j args.size args
+  return fType.instantiateRevRange' j args.size args
 
 def markUsed (n : Nat) (fvars : Array Expr) (b : Expr) (used : Array Bool) : Array Bool := Id.run do
   if !b.hasFVar then return used
@@ -177,8 +177,8 @@ def markUsed (n : Nat) (fvars : Array Expr) (b : Expr) (used : Array Bool) : Arr
 def inferLet (e : Expr) (inferOnly : Bool) : RecM Expr := loop #[] #[] e where
   loop fvars vals : Expr → RecM Expr
   | .letE name type val body _ => do
-    let type := type.instantiateRev fvars
-    let val := val.instantiateRev fvars
+    let type := type.instantiateRev' fvars
+    let val := val.instantiateRev' fvars
     let id := ⟨← mkFreshId⟩
     withLCtx ((← getLCtx).mkLetDecl id name type val) do
       let fvars := fvars.push (.fvar id)
@@ -190,7 +190,7 @@ def inferLet (e : Expr) (inferOnly : Bool) : RecM Expr := loop #[] #[] e where
           throw <| .letTypeMismatch (← getEnv) (← getLCtx) name valType type
       loop fvars vals body
   | e => do
-    let r ← inferType (e.instantiateRev fvars) inferOnly
+    let r ← inferType (e.instantiateRev' fvars) inferOnly
     let r := r.cheapBetaReduce
     let rec loopUsed i (used : Array Bool) :=
       match i with
@@ -449,37 +449,37 @@ def isDefEqLambda (t s : Expr) (subst : Array Expr := #[]) : RecM Bool :=
   match t, s with
   | .lam _ tDom tBody _, .lam name sDom sBody bi => do
     let sType ← if tDom != sDom then
-      let sType := sDom.instantiateRev subst
-      let tType := tDom.instantiateRev subst
+      let sType := sDom.instantiateRev' subst
+      let tType := tDom.instantiateRev' subst
       if !(← isDefEq tType sType) then return false
       pure (some sType)
     else pure none
     if tBody.hasLooseBVars || sBody.hasLooseBVars then
-      let sType := sType.getD (sDom.instantiateRev subst)
+      let sType := sType.getD (sDom.instantiateRev' subst)
       let id := ⟨← mkFreshId⟩
       withLCtx ((← getLCtx).mkLocalDecl id name sType bi) do
         isDefEqLambda tBody sBody (subst.push (.fvar id))
     else
       isDefEqLambda tBody sBody (subst.push default)
-  | t, s => isDefEq (t.instantiateRev subst) (s.instantiateRev subst)
+  | t, s => isDefEq (t.instantiateRev' subst) (s.instantiateRev' subst)
 
 def isDefEqForall (t s : Expr) (subst : Array Expr := #[]) : RecM Bool :=
   match t, s with
   | .forallE _ tDom tBody _, .forallE name sDom sBody bi => do
     let sType ← if tDom != sDom then
-      let sType := sDom.instantiateRev subst
-      let tType := tDom.instantiateRev subst
+      let sType := sDom.instantiateRev' subst
+      let tType := tDom.instantiateRev' subst
       if !(← isDefEq tType sType) then return false
       pure (some sType)
     else pure none
     if tBody.hasLooseBVars || sBody.hasLooseBVars then
-      let sType := sType.getD (sDom.instantiateRev subst)
+      let sType := sType.getD (sDom.instantiateRev' subst)
       let id := ⟨← mkFreshId⟩
       withLCtx ((← getLCtx).mkLocalDecl id name sType bi) do
         isDefEqForall tBody sBody (subst.push (.fvar id))
     else
       isDefEqForall tBody sBody (subst.push default)
-  | t, s => isDefEq (t.instantiateRev subst) (s.instantiateRev subst)
+  | t, s => isDefEq (t.instantiateRev' subst) (s.instantiateRev' subst)
 
 def quickIsDefEq (t s : Expr) (useHash := false) : RecM LBool := do
   if ← modifyGet fun (.mk a1 a2 a3 a4 a5 a6 (eqvManager := m)) =>
@@ -733,18 +733,18 @@ def ensureType (e : Expr) : M Expr := do ensureSort (← inferType e) e
 def etaExpand (e : Expr) : M Expr :=
   let rec loop fvars
   | .lam name dom body bi => do
-    let d := dom.instantiateRev fvars
+    let d := dom.instantiateRev' fvars
     let id := ⟨← mkFreshId⟩
     withLCtx ((← getLCtx).mkLocalDecl id name d bi) do
       let fvars := fvars.push (.fvar id)
       loop fvars body
   | it => do
-    let itType ← whnf <| ← inferType <| it.instantiateRev fvars
+    let itType ← whnf <| ← inferType <| it.instantiateRev' fvars
     if !itType.isForall then return e
     let rec loop2 fvars args
     | 0, _ => throw .deepRecursion
     | fuel + 1, .forallE name dom body bi => do
-      let d := dom.instantiateRev fvars
+      let d := dom.instantiateRev' fvars
       let id := ⟨← mkFreshId⟩
       withLCtx ((← getLCtx).mkLocalDecl id name d bi) do
         let arg := .fvar id
