Lean4Lean/Verify/Typing/Expr.lean
@@ -30,33 +30,36 @@ def VLCtx.WF : VLCtx → Prop
 def TrProj (Γ : List VExpr) (structName : Name) (idx : Nat) (e : VExpr) : VExpr → Prop := sorry
 
 variable (env : VEnv) (Us : List Name) in
-inductive TrExpr : VLCtx → Expr → VExpr → Prop
-  | bvar : Δ.find? (.inl i) = some (e, A) → TrExpr Δ (.bvar i) e
-  | fvar : Δ.find? (.inr fv) = some (e, A) → TrExpr Δ (.fvar fv) e
-  | sort : VLevel.ofLevel Us u = some u' → TrExpr Δ (.sort u) (.sort u')
+inductive TrExprS : VLCtx → Expr → VExpr → Prop
+  | bvar : Δ.find? (.inl i) = some (e, A) → TrExprS Δ (.bvar i) e
+  | fvar : Δ.find? (.inr fv) = some (e, A) → TrExprS Δ (.fvar fv) e
+  | sort : VLevel.ofLevel Us u = some u' → TrExprS Δ (.sort u) (.sort u')
   | const :
     env.constants c = some (some ci) →
     us.mapM (VLevel.ofLevel Us) = some us' →
     us.length = ci.uvars →
-    TrExpr Δ (.const c us) (.const c us')
+    TrExprS Δ (.const c us) (.const c us')
   | app :
     env.HasType Us.length Δ.toCtx f' (.forallE A B) →
     env.HasType Us.length Δ.toCtx a' A →
-    TrExpr Δ f f' → TrExpr Δ a a' → TrExpr Δ (.app f a) (.app f' a')
+    TrExprS Δ f f' → TrExprS Δ a a' → TrExprS Δ (.app f a) (.app f' a')
   | lam :
     env.IsType Us.length Δ.toCtx ty' →
-    TrExpr Δ ty ty' → TrExpr ((none, .vlam ty') :: Δ) body body' →
-    TrExpr Δ (.lam name ty body bi) (.lam ty' body')
+    TrExprS Δ ty ty' → TrExprS ((none, .vlam ty') :: Δ) body body' →
+    TrExprS Δ (.lam name ty body bi) (.lam ty' body')
   | forallE :
     env.IsType Us.length Δ.toCtx ty' →
     env.IsType Us.length (ty' :: Δ.toCtx) body' →
-    TrExpr Δ ty ty' → TrExpr ((none, .vlam ty') :: Δ) body body' →
-    TrExpr Δ (.forallE name ty body bi) (.forallE ty' body')
+    TrExprS Δ ty ty' → TrExprS ((none, .vlam ty') :: Δ) body body' →
+    TrExprS Δ (.forallE name ty body bi) (.forallE ty' body')
   | letE :
     env.HasType Us.length Δ.toCtx val' ty' →
-    TrExpr Δ ty ty' → TrExpr Δ val val' →
-    TrExpr ((none, .vlet ty' val') :: Δ) body body' →
-    TrExpr Δ (.letE name ty val body bi) body'
-  | lit : TrExpr Δ l.toConstructor e → TrExpr Δ (.lit l) e
-  | mdata : TrExpr Δ e e' → TrExpr Δ (.mdata d e) e'
-  | proj : TrExpr Δ e e' → TrProj Δ.toCtx s i e' e'' → TrExpr Δ (.proj s i e) e''
+    TrExprS Δ ty ty' → TrExprS Δ val val' →
+    TrExprS ((none, .vlet ty' val') :: Δ) body body' →
+    TrExprS Δ (.letE name ty val body bi) body'
+  | lit : TrExprS Δ l.toConstructor e → TrExprS Δ (.lit l) e
+  | mdata : TrExprS Δ e e' → TrExprS Δ (.mdata d e) e'
+  | proj : TrExprS Δ e e' → TrProj Δ.toCtx s i e' e'' → TrExprS Δ (.proj s i e) e''
+
+def TrExpr (env : VEnv) (Us : List Name) (Δ : VLCtx) (e : Expr) (e' : VExpr) : Prop :=
+  ∃ e₂, TrExprS env Us Δ e e₂ ∧ env.IsDefEqU Us.length Δ.toCtx e₂ e'
