Lean4Lean/Theory/Typing/UniqueTyping.lean
@@ -8,65 +8,65 @@ A bunch of important structural theorems which we can't prove :(
 namespace Lean4Lean
 namespace VEnv
 
-theorem IsDefEq.uniq (henv : Ordered env) (hΓ : OnCtx Γ (env.IsType U))
+theorem IsDefEq.uniq (henv : VEnv.WF env) (hΓ : OnCtx Γ (env.IsType U))
     (h1 : env.IsDefEq U Γ e₁ e₂ A) (h2 : env.IsDefEq U Γ e₂ e₃ B) :
     ∃ u, env.IsDefEq U Γ A B (.sort u) := sorry
 
-theorem IsDefEq.uniqU (henv : Ordered env) (hΓ : OnCtx Γ (env.IsType U))
+theorem IsDefEq.uniqU (henv : VEnv.WF env) (hΓ : OnCtx Γ (env.IsType U))
     (h1 : env.IsDefEq U Γ e₁ e₂ A) (h2 : env.IsDefEq U Γ e₂ e₃ B) :
     env.IsDefEqU U Γ A B := let ⟨_, h⟩ := h1.uniq henv hΓ h2; ⟨_, h⟩
 
-variable! (henv : Ordered env) in
+variable! (henv : VEnv.WF env) in
 theorem IsDefEqU.weakN (W : Ctx.LiftN n k Γ Γ') (H : env.IsDefEqU U Γ e1 e2) :
     env.IsDefEqU U Γ' (e1.liftN n k) (e2.liftN n k) := let ⟨_, H⟩ := H; ⟨_, H.weakN henv W⟩
 
-theorem isDefEq_iff (henv : Ordered env) (hΓ : OnCtx Γ (env.IsType U)) :
+theorem isDefEq_iff (henv : VEnv.WF env) (hΓ : OnCtx Γ (env.IsType U)) :
     env.IsDefEq U Γ e₁ e₂ A ↔
     env.HasType U Γ e₁ A ∧ env.HasType U Γ e₂ A ∧ env.IsDefEqU U Γ e₁ e₂ := by
   refine ⟨fun h => ⟨h.hasType.1, h.hasType.2, _, h⟩, fun ⟨_, h2, _, h3⟩ => ?_⟩
   have ⟨_, h⟩ := h3.uniq henv hΓ h2
   exact h.defeqDF h3
 
-theorem IsDefEq.trans_r (henv : Ordered env) (hΓ : OnCtx Γ (env.IsType U))
+theorem IsDefEq.trans_r (henv : VEnv.WF env) (hΓ : OnCtx Γ (env.IsType U))
     (h₁ : env.IsDefEq U Γ e₁ e₂ A) (h₂ : env.IsDefEq U Γ e₂ e₃ B) :
     env.IsDefEq U Γ e₁ e₃ B := by
   have ⟨_, h⟩ := h₁.uniq henv hΓ h₂
   exact .trans (.defeqDF h h₁) h₂
 
-theorem IsDefEq.trans_l (henv : Ordered env) (hΓ : OnCtx Γ (env.IsType U))
+theorem IsDefEq.trans_l (henv : VEnv.WF env) (hΓ : OnCtx Γ (env.IsType U))
     (h₁ : env.IsDefEq U Γ e₁ e₂ A) (h₂ : env.IsDefEq U Γ e₂ e₃ B) :
     env.IsDefEq U Γ e₁ e₃ A := by
   have ⟨_, h⟩ := h₁.uniq henv hΓ h₂
   exact h₁.trans (.defeqDF (.symm h) h₂)
 
-theorem IsDefEqU.defeqDF (henv : Ordered env) (hΓ : OnCtx Γ (env.IsType U))
+theorem IsDefEqU.defeqDF (henv : VEnv.WF env) (hΓ : OnCtx Γ (env.IsType U))
     (h₁ : env.IsDefEqU U Γ A B) (h₂ : env.IsDefEq U Γ e₁ e₂ A) :
     env.IsDefEq U Γ e₁ e₂ B := by
   have ⟨_, h₁⟩ := h₁
   have ⟨_, hA⟩ := h₂.isType henv hΓ
   exact .defeqDF (hA.trans_l henv hΓ h₁) h₂
 
-theorem IsDefEqU.of_l (henv : Ordered env) (hΓ : OnCtx Γ (env.IsType U))
+theorem IsDefEqU.of_l (henv : VEnv.WF env) (hΓ : OnCtx Γ (env.IsType U))
     (h1 : env.IsDefEqU U Γ e₁ e₂) (h2 : env.HasType U Γ e₁ A) :
     env.IsDefEq U Γ e₁ e₂ A := let ⟨_, h⟩ := h1; h2.trans_l henv hΓ h
 
-theorem HasType.defeqU_l (henv : Ordered env) (hΓ : OnCtx Γ (env.IsType U))
+theorem HasType.defeqU_l (henv : VEnv.WF env) (hΓ : OnCtx Γ (env.IsType U))
     (h1 : env.IsDefEqU U Γ e₁ e₂) (h2 : env.HasType U Γ e₁ A) :
     env.HasType U Γ e₂ A := (h1.of_l henv hΓ h2).hasType.2
 
-theorem IsType.defeqU_l (henv : Ordered env) (hΓ : OnCtx Γ (env.IsType U))
+theorem IsType.defeqU_l (henv : VEnv.WF env) (hΓ : OnCtx Γ (env.IsType U))
     (h1 : env.IsDefEqU U Γ A₁ A₂) (h2 : env.IsType U Γ A₁) :
     env.IsType U Γ A₂ := h2.imp fun _ h2 => h2.defeqU_l henv hΓ h1
 
-theorem IsDefEqU.of_r (henv : Ordered env) (hΓ : OnCtx Γ (env.IsType U))
+theorem IsDefEqU.of_r (henv : VEnv.WF env) (hΓ : OnCtx Γ (env.IsType U))
     (h1 : env.IsDefEqU U Γ e₁ e₂) (h2 : env.HasType U Γ e₂ A) :
     env.IsDefEq U Γ e₁ e₂ A := (h1.symm.of_l henv hΓ h2).symm
 
-theorem HasType.defeqU_r (henv : Ordered env) (hΓ : OnCtx Γ (env.IsType U))
+theorem HasType.defeqU_r (henv : VEnv.WF env) (hΓ : OnCtx Γ (env.IsType U))
     (h1 : env.IsDefEqU U Γ A₁ A₂) (h2 : env.HasType U Γ e A₁) :
     env.HasType U Γ e A₂ := h1.defeqDF henv hΓ h2
 
-theorem IsDefEqU.trans (henv : Ordered env) (hΓ : OnCtx Γ (env.IsType U))
+theorem IsDefEqU.trans (henv : VEnv.WF env) (hΓ : OnCtx Γ (env.IsType U))
     (h1 : env.IsDefEqU U Γ e₁ e₂) (h2 : env.IsDefEqU U Γ e₂ e₃) :
     env.IsDefEqU U Γ e₁ e₃ := h1.imp fun _ h1 => let ⟨_, h2⟩ := h2; h1.trans_l henv hΓ h2
 
