Lean4Lean/Verify/Expr.lean
@@ -1,0 +1,166 @@
+import Lean4Lean.Std.Basic
+import Lean4Lean.Verify.Axioms
+import Lean4Lean.Expr
+import Lean4Lean.Instantiate
+import Lean
+
+namespace Lean
+namespace Expr
+
+theorem mkData_looseBVarRange (H : br ≤ 2^20 - 1) :
+    (mkData h br d fv ev lv lp).looseBVarRange.toNat = br := by
+  rw [mkData, if_pos H]; dsimp only [Data.looseBVarRange, -Nat.reducePow]
+  have : br.toUInt64.toUInt32.toNat = br := by simp; omega
+  refine .trans ?_ this; congr 2
+  refine UInt64.eq_of_toBitVec_eq ?_
+  have : br.toUInt64.toNat = br := by simp; omega
+  have : br.toUInt64.toBitVec ≤ 0xfffff#64 := (this ▸ H :)
+  have : h.toUInt32.toUInt64.toBitVec ≤ 0xffffffff#64 :=
+    show h.toUInt32.toNat ≤ 2^32-1 by simp; omega
+  have : (if d > 255 then 255 else d.toUInt8).toUInt64.toBitVec ≤ 0xff#64 :=
+    Nat.le_of_lt_succ (if d > 255 then 255 else d.toUInt8).1.1.2
+  have hb : ∀ (b : Bool), b.toUInt64.toBitVec ≤ 1#64 := by decide
+  have := hb fv; have := hb ev; have := hb lv; have := hb lp
+  change
+    (h.toUInt32.toUInt64.toBitVec +
+      (if d > 255 then 255 else d.toUInt8).toUInt64.toBitVec <<< 32#64 +
+      fv.toUInt64.toBitVec <<< 40#64 +
+      ev.toUInt64.toBitVec <<< 41#64 +
+      lv.toUInt64.toBitVec <<< 42#64 +
+      lp.toUInt64.toBitVec <<< 43#64 +
+      br.toUInt64.toBitVec <<< 44#64) >>> 44#64 =
+    br.toUInt64.toBitVec
+  bv_decide
+
+theorem Data.looseBVarRange_le : (Data.looseBVarRange d).toNat ≤ 2^20 - 1 := by
+  rw [Data.looseBVarRange]
+  suffices (UInt64.shiftRight d 44).toNat ≤ 2 ^ 20 - 1 by simp; omega
+  show d.toBitVec >>> 44#64 ≤ 0xfffff#64
+  bv_decide
+
+theorem looseBVarRange_le : looseBVarRange e ≤ 2^20 - 1 := Data.looseBVarRange_le
+
+theorem _root_.UInt32.max_toNat (a b : UInt32) : (max a b).toNat = max a.toNat b.toNat := by
+  simp only [instMaxUInt32, maxOfLe, UInt32.le_iff_toNat_le, Nat.instMax]; split <;> rfl
+
+theorem mkAppData_looseBVarRange :
+    (mkAppData fData aData).looseBVarRange = max fData.looseBVarRange aData.looseBVarRange := by
+  have hm : max fData.looseBVarRange aData.looseBVarRange ≤ (Nat.pow 2 20 - 1).toUInt32 := by
+    dsimp [instMaxUInt32, maxOfLe]; split <;> exact Data.looseBVarRange_le
+  rw [mkAppData, if_pos hm]
+  simp [Data.looseBVarRange] at hm
+  dsimp only [Data.looseBVarRange, -Nat.reducePow]
+  generalize (max .. : UInt32) = m at *
+  have : m.toUInt64.toUInt32 = m := by simp [UInt64.toUInt32]
+  refine .trans ?_ this; congr 2
+  generalize (ite (_ > (255 : UInt16)) _ _ : UInt8) = a
+  generalize HOr.hOr (α := UInt64) fData _ = b
+  generalize UInt64.toUInt32 _ = c
+  apply UInt64.eq_of_toBitVec_eq
+  change m.toUInt64.toBitVec ≤ 0xfffff#64 at hm
+  have : c.toUInt64.toBitVec ≤ 0xffffffff#64 := Nat.le_of_lt_succ c.1.1.2
+  have : a.toUInt64.toBitVec ≤ 0xff#64 := Nat.le_of_lt_succ a.1.1.2
+  change
+    (b.toBitVec &&& 15#64 <<< 40#64 |||
+      c.toUInt64.toBitVec |||
+      a.toUInt64.toBitVec <<< 32#64 |||
+      m.toUInt64.toBitVec <<< 44#64) >>> 44#64 =
+    m.toUInt64.toBitVec
+  bv_decide
+
+theorem Safe.looseBVarRange_eq :
+    ∀ {e}, Safe e → e.looseBVarRange = e.realLooseBVarRange
+  | .bvar i, e => by simp [looseBVarRange, data]; rw [mkData_looseBVarRange e]; rfl
+  | .const .., _
+  | .sort _, _
+  | .fvar _, _
+  | .mvar _, _
+  | .lit _, _ => mkData_looseBVarRange (Nat.zero_le _)
+  | .mdata _ e, h
+  | .proj _ _ e, h =>
+    (mkData_looseBVarRange looseBVarRange_le).trans <| h.looseBVarRange_eq (e := e)
+  | .app e1 e2, ⟨h1, h2⟩ => by
+    simp [looseBVarRange, Expr.data, mkAppData_looseBVarRange, UInt32.max_toNat,
+      realLooseBVarRange, ← h1.looseBVarRange_eq, ← h2.looseBVarRange_eq]
+  | .lam _ e1 e2 _, ⟨h1, h2⟩
+  | .forallE _ e1 e2 _, ⟨h1, h2⟩ => by
+    simp [looseBVarRange, Expr.data, Expr.mkDataForBinder, realLooseBVarRange]
+    rw [mkData_looseBVarRange, ← h1.looseBVarRange_eq, ← h2.looseBVarRange_eq]; · rfl
+    exact Nat.max_le.2 ⟨looseBVarRange_le, Nat.le_trans (Nat.sub_le ..) looseBVarRange_le⟩
+  | .letE _ e1 e2 e3 _, ⟨h1, h2, h3⟩ => by
+    simp [looseBVarRange, Expr.data, Expr.mkDataForLet, realLooseBVarRange]
+    rw [mkData_looseBVarRange, ← h1.looseBVarRange_eq, ← h2.looseBVarRange_eq,
+      ← h3.looseBVarRange_eq]; · rfl
+    exact Nat.max_le.2 ⟨
+      Nat.max_le.2 ⟨looseBVarRange_le, looseBVarRange_le⟩,
+      Nat.le_trans (Nat.sub_le ..) looseBVarRange_le⟩
+
+theorem Safe.getAppFn {e} (h : Safe e) : Safe e.getAppFn := by
+  unfold Expr.getAppFn; split
+  · exact h.1.getAppFn
+  · exact h
+
+def getAppArgsRevList : Expr → List Expr
+  | .app f a => a :: f.getAppArgsRevList
+  | _ => []
+
+open private getAppNumArgsAux getAppArgsAux mkAppRangeAux from Lean.Expr
+
+theorem getAppNumArgs_eq : getAppNumArgs e = (getAppArgsRevList e).length := by
+  let rec loop e n : getAppNumArgsAux e n = (getAppArgsRevList e).length + n := by
+    unfold getAppNumArgsAux getAppArgsRevList; split <;> simp
+    rw [loop]; omega
+  rw [getAppNumArgs, loop]; rfl
+
+theorem getAppArgs_toList : (getAppArgs e).toList = (getAppArgsRevList e).reverse := by
+  let rec loop {e l₁ l₂ args} (h1 : args.toList = l₁ ++ l₂) :
+      l₁.length = (getAppArgsRevList e).length →
+      (getAppArgsAux e args ((getAppArgsRevList e).length - 1)).toList =
+      (getAppArgsRevList e).reverse ++ l₂ := by
+    unfold getAppArgsAux getAppArgsRevList; split
+    · rename_i f a; intro h2
+      obtain rfl | ⟨l₁, u, rfl⟩ := List.eq_nil_or_concat l₁; · cases h2
+      simp at h2 ⊢; refine loop ?_ h2
+      simp [← h2, h1]
+    · simp; rintro ⟨⟩; simpa using h1
+  simp [getAppArgs, getAppNumArgs_eq]
+  exact (loop (List.append_nil _).symm (by simp)).trans (by simp)
+
+theorem getAppArgs_eq : getAppArgs e = (getAppArgsRevList e).reverse.toArray := by
+  simp [← getAppArgs_toList]
+
+@[simp] def mkAppRevList : Expr → List Expr → Expr
+  | e, [] => e
+  | e, a :: as => .app (mkAppRevList e as) a
+
+theorem mkAppRevList_eq_foldr : mkAppRevList e es = es.foldr (fun a e => .app e a) e := by
+  induction es <;> simp [mkAppRevList, *]
+
+@[simp] theorem mkAppRevList_append :
+    mkAppRevList e (es₁ ++ es₂) = mkAppRevList (mkAppRevList e es₂) es₁ := by
+  simp [mkAppRevList_eq_foldr]
+
+theorem mkAppRevList_getAppArgsRevList (e) :
+    mkAppRevList e.getAppFn (getAppArgsRevList e) = e := by
+  unfold getAppFn getAppArgsRevList; split <;> simp
+  congr 1; exact mkAppRevList_getAppArgsRevList _
+
+theorem mkAppRange_eq (h1 : args.toList = l₁ ++ l₂ ++ l₃)
+    (h2 : l₁.length = i) (h3 : (l₁ ++ l₂).length = j) :
+    mkAppRange e i j args = mkAppRevList e l₂.reverse := loop h1 h2 h3 where
+  loop {n i e l₁ l₂} (h1 : args.toList = l₁ ++ l₂ ++ l₃)
+      (h2 : l₁.length = i) (h3 : (l₁ ++ l₂).length = n) :
+      mkAppRangeAux n args i e = mkAppRevList e l₂.reverse := by
+    rw [mkAppRangeAux.eq_def]; split
+    · simp [Array.get!, ← Array.getElem?_toList, h1]
+      obtain _ | ⟨a, l₂⟩ := l₂; · simp_all
+      rw [List.getElem?_append_right (by simp [h2])]
+      simp [h2]
+      rw [loop (l₁ := l₁ ++ [a]) (l₂ := l₂)] <;> simp [h1, h2, h3, mkApp]
+    · simp at h3
+      have : l₂.length = 0 := by omega
+      simp at this; simp [this]
+
+@[simp] def instantiateList : Expr → List Expr → Expr
+  | e, [] => e
+  | e, a :: as => instantiateList (e.instantiate1' a) as
