Lean4Lean/Verify/Typing/ConditionallyTyped.lean
@@ -5,7 +5,7 @@ open VEnv Lean
 
 def ConditionallyTyped
     (ngen : NameGenerator) (env : VEnv) (Us : List Name) (Δ : VLCtx) (e : Expr) : Prop :=
-  InScope ngen.Reserves e ∧ (InScope (· ∈ Δ.fvars) e → ∃ e', TrExpr env Us Δ e e')
+  InScope ngen.Reserves e ∧ (InScope (· ∈ Δ.fvars) e → ∃ e', TrExprS env Us Δ e e')
 
 theorem ConditionallyTyped.mono (H : ngen₁ ≤ ngen₂) :
     ConditionallyTyped ngen₁ env Us Δ e → ConditionallyTyped ngen₂ env Us Δ e
@@ -17,7 +17,7 @@ theorem ConditionallyTyped.weakN_inv
     ConditionallyTyped ngen env Us Δ e := by
   refine H.imp_right fun H1 H2 => ?_
   have ⟨e', H⟩ := H1 H2.fvars_cons
-  exact TrExpr.weakN_inv henv (.skip_fvar _ _ .refl) (.refl henv hΔ) H H2
+  exact TrExprS.weakN_inv henv (.skip_fvar _ _ .refl) (.refl henv hΔ) H H2
 
 theorem ConditionallyTyped.fresh
     (henv : Ordered env) (hΔ : VLCtx.WF env Us.length ((some ⟨ngen.curr⟩, d) :: Δ))
@@ -31,7 +31,7 @@ theorem ConditionallyTyped.fresh
 
 def TrHasType (env : VEnv) (Us : List Name) (Δ : VLCtx) (e A : Expr) : Prop :=
   (∀ P, IsFVarUpSet P Δ → InScope P e → InScope P A) ∧
-  ∃ e' A', TrExpr env Us Δ e e' ∧ TrExpr env Us Δ A A' ∧ env.HasType Us.length Δ.toCtx e' A'
+  ∃ e' A', TrExprS env Us Δ e e' ∧ TrExprS env Us Δ A A' ∧ env.HasType Us.length Δ.toCtx e' A'
 
 def ConditionallyHasType
     (ngen : NameGenerator) (env : VEnv) (Us : List Name) (Δ : VLCtx) (e A : Expr) : Prop :=
@@ -54,10 +54,10 @@ theorem ConditionallyHasType.weakN_inv
   refine ⟨H1, H2, fun H4 => ?_⟩
   have ⟨h1, e', A', h2, h3, h4⟩ := H3 H4.fvars_cons
   have W : VLCtx.LiftN Δ ((some fv, d) :: Δ) 0 (0 + d.depth) 0 := .skip_fvar _ _ .refl
-  have ⟨e'', he⟩ := TrExpr.weakN_inv henv W (.refl henv hΔ) h2 H4
+  have ⟨e'', he⟩ := TrExprS.weakN_inv henv W (.refl henv hΔ) h2 H4
   have ee := h2.uniq henv (.refl henv hΔ) <| he.weakN henv W hΔ
   have : IsFVarUpSet (· ∈ VLCtx.fvars Δ) ((some fv, d) :: Δ) := ⟨(hΔ.2.1 _ rfl).elim, .fvars⟩
-  have ⟨_, hA⟩ := TrExpr.weakN_inv henv W (.refl henv hΔ) h3 <| h1 _ this H4
+  have ⟨_, hA⟩ := TrExprS.weakN_inv henv W (.refl henv hΔ) h3 <| h1 _ this H4
   have AA := h3.uniq henv (.refl henv hΔ) <| hA.weakN henv W hΔ
   have h4 := h4.defeqU_r henv hΔ.toCtx AA |>.defeqU_l henv hΔ.toCtx ee
   have h4 := (HasType.weakN_iff henv hΔ.toCtx W.toCtx).1 h4
